more legible

main.v
@@ -1,23 +1,34 @@
 Require Import Arith.
+Require Import Basics.
+ (* for composition *)
+Open Scope program_scope.
 Open Scope list_scope.
 
 Set Implicit Arguments.
 Unset Strict Implicit.
 Unset Printing Implicit Defensive.
 
-(* Signatures could alternatively be defined as { A : Type & A -> list nat} *)
-Record sig :=  { O : Type;
-                 ar : O -> list nat}.
+(* Class has_substitution (X : Type) := substitution : (nat -> X) -> (X -> X). *)
+(* Notation "x [ s ]" := (substitution s x) (at level 30). *)
 
-Inductive O_LC :=
-  App | Abs.
-Definition sig_LC : sig :=
+(* substitution in a model *)
+Reserved Notation "x [ s ]" (at level 30).
+(* substitution in the syntax *)
+Reserved Notation "x [ s ]ₛ" (at level 30).
+
+
+Record signature :=
+  { O  : Type;
+    ar : O -> list nat}.
+
+Inductive O_LC := App | Abs.
+
+Definition signature_LC : signature :=
   {| O := O_LC;
      ar := fun o => match o with
                    App => 0 :: 0 :: nil
                  | Abs => 1 :: nil
                  end
-
   |}.
 
 (* Vec {A} B l is a B-list of the same size as l *)
@@ -26,11 +37,11 @@ Inductive Vec {A : Type} (B : Type) : list A -> Type :=
   | ConsV : forall a lA, B -> Vec B lA -> Vec B (a :: lA).
 
 
-Inductive Z (Sig : sig) : Type :=
-  Var : nat -> Z Sig
-| Op : forall (o : O Sig), Vec (Z Sig) (ar o) (* this is Z^(length ar) *) -> Z Sig.
+Inductive Z (S : signature) : Type :=
+  Var : nat -> Z S
+| Op : forall (o : O S), Vec (Z S) (ar o) (* this is Z^(length ar) *) -> Z S.
 
-Arguments Op [Sig] o.
+Arguments Op [S] o.
 
 Definition Vec_map {A B C : Type}(f : A -> B -> C) :=
   fix rec (l : list A) (v : Vec B l) : Vec C l :=
@@ -50,74 +61,155 @@ Definition vec_map_fun_ext {A B C : Type}(f g : A -> B -> C) {l : list A}
 Defined.
 
 
+(* shifts on renamings *)
+Definition shiftₙ (n : nat) (f : nat -> nat)  : nat -> nat :=
+    fun p => if p <? n then p else f (p - n) + n.
 
-Fixpoint Z_ren {Sig : sig}  (f : nat -> nat) (x : Z Sig) {struct x} : Z Sig :=
+
+(* shifts on substitution using renamings *)
+Definition shiftₙₛ {X : Type}(var : nat -> X)(ren : (nat -> nat) -> (X -> X))(n : nat) (f : nat -> X)  : nat -> X :=
+    fun p => if p <? n then var p else ren (fun x => x + n) (f (p - n)).
+
+(* shifts on substitution using substitution structure *)
+Definition shiftₛ {X : Type}(var : nat -> X)(subst : (nat -> X) -> (X -> X))(n : nat) (f : nat -> X)  : nat -> X :=
+  shiftₙₛ var (fun f => subst (fun n => var (f n))) n f.
+
+Lemma commutes_if {A B : Type}(f : A -> B)(b : bool) x y :
+  (if b then f x else f y) = f (if b then x else y).
+Proof.
+destruct b; reflexivity.
+Qed.
+
+Lemma shiftₙₛ_natural
+      {X : Type} (varX : nat -> X) (renX : (nat -> nat) -> (X -> X))
+      {Y : Type} (varY : nat -> Y) (renY : (nat -> nat) -> (Y -> Y))
+      (g : X -> Y)(gvar : forall n, g (varX n) = varY n)
+        (gren : forall f x, g (renX f x) = renY f (g x))
+      (n : nat) (f : nat -> X) x :
+  g (shiftₙₛ varX renX n f x) = shiftₙₛ varY renY n (fun n => g (f n)) x.
+Proof.
+  unfold shiftₙ, shiftₙₛ.
+  rewrite <- gvar, <- gren.
+  symmetry.
+  apply commutes_if.
+Qed.
+
+Lemma var_shiftₙ 
+      {X : Type}(var : nat -> X)(ren : (nat -> nat) -> (X -> X))
+      (eq_ren : forall f n, ren f (var n) = var (f n))
+      (n : nat) (f : nat -> nat) (x : nat) :
+  var ((shiftₙ n f) x) = shiftₙₛ var ren n (fun p => var (f p)) x.
+Proof.
+  unfold shiftₙ.
+  etransitivity; revgoals.
+  eapply  (shiftₙₛ_natural (g := var)).
+  - reflexivity.
+  - symmetry.
+    apply eq_ren.
+  - reflexivity.
+Qed.
+  
+Lemma shiftₙₛ_ext {X : Type}(var : nat -> X)(ren ren' : (nat -> nat) -> (X -> X))
+      (ren_eq : forall f x, ren f x = ren' f x)
+      (n : nat) (f g : nat -> X)
+      (fg_eq : forall p, f p = g p) p : shiftₙₛ var ren n f p = 
+                                   shiftₙₛ var ren' n g p .
+Proof.
+  unfold shiftₙₛ.
+  rewrite fg_eq, ren_eq.
+  reflexivity.
+Qed.
+
+(** Renaming *)
+Fixpoint Z_ren {S : signature}  (f : nat -> nat) (x : Z S) {struct x} : Z S :=
   match x with
     Var _ n => Var _ (f n)
-  | Op op  v => Op op (Vec_map (fun n b => (Z_ren (fun p => if p <? n then p else f (p - n) + n) b))  v)
+  | Op op  v => Op op (Vec_map (fun n b => (Z_ren (shiftₙ n f) b))  v)
   end.
 
-Fixpoint Z_subst {Sig : sig}  (f : nat -> Z Sig) (x : Z Sig) : Z Sig :=
+
+
+(** Substitution *)
+Fixpoint Z_subst {S : signature}  (f : nat -> Z S) (x : Z S) : Z S :=
   match x with
     Var _ n => f n
   | Op op v => Op op
-                        (Vec_map 
-                           (fun n b => (Z_subst (fun p => if p <? n then Var Sig p else Z_ren (fun x => x + n) (f (p - n))) b)
-                        ) v)
-    end.
+                 (Vec_map 
+                    (fun n b =>
+                       (b [ shiftₙₛ (Var S) Z_ren n f ]ₛ)
+                    ) v)
+  end
+    where "t [ f ]ₛ" := (Z_subst f t).
+
+(* Instance Z_has_substitution (S : signature) : has_substitution (Z S) := Z_subst. *)
 
 
-Record model_data (Sig : sig) := 
+Record model_data (S : signature) := 
   { carrier :> Type;
     variables : nat -> carrier;
-    ops : forall (o : O Sig), Vec carrier (ar o) -> carrier;
-    substitution : (nat -> carrier) -> carrier -> carrier ;
-  }.
-Arguments ops [Sig m] o.
+    ops : forall (o : O S), Vec carrier (ar o) -> carrier;
+    (* has_subst :> has_substitution carrier *)
+    substitution : (nat -> carrier) -> (carrier -> carrier)
 
-Record model_laws {Sig : sig}(m : model_data Sig) :=
+  }.
+
+Arguments ops [S m] o.
+Notation "x [ s ]" := (substitution s x).
+Notation "↑" := (shiftₛ (variables _) (substitution (m := _))).
+(* Existing Instance has_subst . *)
+
+Record model_laws {S : signature}(m : model_data S) :=
   {
     (* fun ext for substitution *)
     substitution_ext : forall (f g : nat -> m),  (forall n, f n = g n) -> forall x,
-                                    substitution f x = substitution g x;
-    variables_eq : forall x f, substitution f (variables m x) = f x;
+                                    x [ f ] = x [ g ] ;
+    variables_eq : forall x f, (variables m x) [ f ] = f x;
     (* operations are module morphisms *)
-    ops_eq : forall (o : O Sig)
+    ops_eq : forall (o : O S)
                (v : Vec m (ar o))
                (f : nat -> m),
           substitution f (ops o v) =
           ops o (Vec_map
-                        (fun n =>
-                           substitution
-                             (fun x => if x <? n then variables m x else
-                                         substitution (fun p => variables m (p + n)) (f (x - n)))) v)
-    (* missing laws: associativity of substitution *) ;
+                        (fun n t =>
+                           (* substitution (shiftₛ (variables m) substitution n f)) *)
+                           (* substitution (shiftₛ (variables m) (substitution (m := m)) n f) *)
+                           t [ ↑ n f ]
+                        )
+              v);
+
+    (* additionnal laws (not needed for initiality) : associativity of substitution *) 
     assoc : forall (f g : nat -> m) (x : m),
-        substitution f (substitution g x) = substitution (fun n => substitution f (g n)) x ;
-    id_neutral : forall (x : m), substitution (variables m) x = x
+        x [ g ] [ f ] = x [ (fun n => (g n) [ f ]) ] ;
+    id_neutral : forall (x : m), x [ variables m ] = x
   }.
 
-Record model (Sig : sig) :=
-  { data :> model_data Sig;
+Record model (S : signature) :=
+  { data :> model_data S;
     laws : model_laws data
   }.
 
-Record model_mor {Sig : sig} (X : model Sig) (Y : model Sig) :=
+Record model_mor {S : signature} (X : model S) (Y : model S) :=
   { carrier_mor :> X -> Y ;
     variables_mor : forall n, carrier_mor (variables X n) = variables Y n ;
-    substitution_mor : forall (f : nat -> X) (x : X), carrier_mor (substitution f x) =
-                                              substitution (fun n => carrier_mor (f n))
-                                                           (carrier_mor x) ;
-    ops_mor : forall (o : O Sig)(v : Vec X (ar o)), carrier_mor (ops o v) =
+    substitution_mor : forall (f : nat -> X) (x : X), carrier_mor (x [ f ]) =
+                                              (carrier_mor x) [ carrier_mor ∘ f ];
+    ops_mor : forall (o : O S)(v : Vec X (ar o)), carrier_mor (ops o v) =
                                                          ops o (Vec_map (fun _ => carrier_mor) v)
   
   }.
 
 (* Z is a model *)
 
+Definition Z_model_data (S : signature) : model_data S :=
+  {|
+  carrier := Z S;
+  variables := Var S;
+  ops := @Op S;
+  substitution := Z_subst
+ |}.
 
-Fixpoint Z_subst_funext {Sig}(f g : nat -> Z Sig) (eq : forall n, f n = g n) x :
-  Z_subst f x = Z_subst g x.
+Fixpoint Z_subst_ext {S}(f g : nat -> Z S) (eq : forall n, f n = g n) x :
+  x [ f ]ₛ = x [ g ]ₛ.
 Proof.
   destruct x.
   - cbn; apply eq.
@@ -125,14 +217,15 @@ Proof.
     f_equal.
     apply vec_map_fun_ext.
     intros.
-    apply Z_subst_funext.
+    apply Z_subst_ext.
     intro.
-    rewrite eq.
-    reflexivity.
+    eapply shiftₙₛ_ext.
+    + reflexivity.
+    + apply eq.
 Qed.
 
-Fixpoint Z_ren_subst_eq {Sig} (f : nat -> nat) (x : Z Sig) :
-  Z_ren f x = Z_subst (fun n => Var Sig (f n)) x.
+Fixpoint Z_ren_subst_eq {S} (f : nat -> nat) (x : Z S) :
+  Z_ren f x = x [ fun n => Var S (f n) ]ₛ.
 Proof.
   destruct x.
   - reflexivity.
@@ -142,34 +235,20 @@ Proof.
     intros.
     rewrite Z_ren_subst_eq.
     cbn.
-    apply Z_subst_funext.
+    apply Z_subst_ext.
     intro.
-    destruct a; [reflexivity|].
-    destruct (n <=? a); reflexivity.
+    apply var_shiftₙ.
+    reflexivity.
 Qed.
-          
-Definition Z_model_data (Sig : sig) : model_data Sig :=
-  {|
-  carrier := Z Sig;
-  variables := Var Sig;
-  ops := @Op Sig;
-  substitution := Z_subst
- |}.
 
-
-Lemma commutes_if {A B : Type}(f : A -> B)(b : bool) x y :
-  (if b then f x else f y) = f (if b then x else y).
-Proof.
-destruct b; reflexivity.
-Qed.
 
 (* Uniqueness of the renamings *)
-Fixpoint ZModel_unique_ren (Sig : sig) (s : (nat -> Z Sig) -> Z Sig -> Z Sig)
-      (s_laws : model_laws {| carrier := Z Sig;
-                              variables := Var Sig;
-                              ops := @Op Sig;
+Fixpoint ZModel_unique_ren (S : signature) (s : (nat -> Z S) -> Z S -> Z S)
+      (s_laws : model_laws {| carrier := Z S;
+                              variables := Var S;
+                              ops := @Op S;
                               substitution := s|}) f z {struct z} :
-    s (fun n => Var Sig (f n)) z = Z_ren f z.
+    s (fun n => Var S (f n)) z = Z_ren f z.
 Proof.
   intros.
   destruct z.
@@ -183,19 +262,21 @@ Proof.
     etransitivity. 
     {  apply (substitution_ext s_laws).
        intro n.
-       rewrite (variables_eq s_laws (f (n - a))). 
-       apply (commutes_if (Var Sig)).
+       etransitivity;[symmetry; apply var_shiftₙ|].
+       intros.
+       exact (variables_eq s_laws _ _).
+       reflexivity.
     }
     apply (ZModel_unique_ren _ _ s_laws).
 Qed.
 
 (* Uniqueness of the substitution *)
-Fixpoint ZModel_unique_subst (Sig : sig) (s : (nat -> Z Sig) -> Z Sig -> Z Sig)
-      (s_laws : model_laws {| carrier := Z Sig;
-                              variables := Var Sig;
-                              ops := @Op Sig;
+Fixpoint ZModel_unique_subst (S : signature) (s : (nat -> Z S) -> Z S -> Z S)
+      (s_laws : model_laws {| carrier := Z S;
+                              variables := Var S;
+                              ops := @Op S;
                               substitution := s|}) f z {struct z} :
-    s f z = Z_subst f z.
+    s f z = z [ f ]ₛ. 
 Proof.
   intros.
   destruct z.
@@ -208,24 +289,26 @@ Proof.
     intros.
     etransitivity.
     apply (ZModel_unique_subst _ _ s_laws).
-    apply Z_subst_funext.
+    apply Z_subst_ext.
     intro n.
-    rewrite (ZModel_unique_ren s_laws).
-    reflexivity.
+    apply shiftₙₛ_ext.
+    + apply (ZModel_unique_ren s_laws).
+    + reflexivity.
 Qed.
 
 
-Lemma Z_model_laws (Sig : sig) : model_laws (Z_model_data Sig).
+Lemma Z_model_laws (S : signature) : model_laws (Z_model_data S).
 Proof.
   repeat split.
-  - exact Z_subst_funext.
+  - exact Z_subst_ext.
   - cbn.
     intros o v f.
     f_equal.
     apply vec_map_fun_ext.
     intros.
-    apply Z_subst_funext.
+    apply Z_subst_ext.
     intro.
+    unfold shiftₙₛ.
     rewrite Z_ren_subst_eq.
     reflexivity.
   - admit.
@@ -233,20 +316,20 @@ Proof.
 
 Admitted.
 
-Definition ZModel (Sig : sig) : model Sig :=
-  {| data := Z_model_data Sig; laws := Z_model_laws Sig |}.
+Definition ZModel (S : signature) : model S :=
+  {| data := Z_model_data S; laws := Z_model_laws S |}.
 
 (* the initial morphism *)
 
-Fixpoint ini_mor {Sig : sig} (m : model Sig )(x : Z Sig) : m :=
+Fixpoint ini_mor {S : signature} (m : model S )(x : Z S) : m :=
   match x with
         Var _ n => variables _ n
       | Op o v   => ops o (Vec_map (fun _ => ini_mor m) v)
   end.
 
 (* the initial morphism preserves renaming *)
-Fixpoint mor_ren { Sig : sig}(m : model Sig)(f : nat -> nat) (x : Z Sig) :
-  ini_mor m (Z_ren f x) = substitution (fun y => variables _ (f y)) (ini_mor m x).
+Fixpoint mor_ren { S : signature}(m : model S)(f : nat -> nat) (x : Z S) :
+  ini_mor m (Z_ren f x) = (ini_mor m x) [ variables m ∘ f ].
   destruct x as [n|o v].
   - cbn.
     rewrite (variables_eq (laws m)).
@@ -266,16 +349,19 @@ Fixpoint mor_ren { Sig : sig}(m : model Sig)(f : nat -> nat) (x : Z Sig) :
         cbn -[leb].
         apply (substitution_ext (laws m)).
         intro n.
-        destruct (n <? a).
-        --  reflexivity.
-        --  rewrite (variables_eq (laws m)).
-            reflexivity.
+        unfold compose.
+        apply var_shiftₙ.
+        cbn.
+        intros.
+        rewrite (variables_eq (laws m)).
+        reflexivity.
 Defined.
 
 
 (* the initial morphism preserves substitution *)
-Fixpoint mor_subst {Sig : sig}(m : model Sig)(f : nat -> Z Sig) (x : Z Sig) :
-  ini_mor m (Z_subst f x) = substitution (fun y => ini_mor m (f y)) (ini_mor m x).
+Fixpoint mor_subst {S : signature}(m : model S)(f : nat -> Z S) (x : Z S) :
+  (* ini_mor m (x [ f ]ₛ) = (ini_mor m x) [fun y => ini_mor m (f y)]. *)
+  ini_mor m (x [ f ]ₛ) = (ini_mor m x) [ ini_mor m ∘ f].
   destruct x as [n|o v].
   - cbn.
     rewrite (variables_eq (laws m)).
@@ -290,18 +376,19 @@ Fixpoint mor_subst {Sig : sig}(m : model Sig)(f : nat -> Z Sig) (x : Z Sig) :
     + cbn -[leb].
       f_equal; revgoals.
       * exact IHv.
-      * cbn -[leb].
-        rewrite mor_subst.
-        cbn -[leb].
+      * rewrite mor_subst.
         apply (substitution_ext (laws m)).
         intro n.
-        destruct (n <? a).
-        --  reflexivity.
-        --  apply mor_ren.
-Defined.
+        unfold compose.
+        apply shiftₙₛ_natural.
+        -- reflexivity.
+        -- intros.
+           apply mor_ren.
+Qed.
 
 
-Program Definition initial_morphism {Sig : sig}(m : model Sig) : model_mor (ZModel Sig) m :=
+
+Program Definition initial_morphism {S : signature}(m : model S) : model_mor (ZModel S) m :=
   {|
   carrier_mor := ini_mor m;
   |}.
@@ -309,7 +396,7 @@ Next Obligation.
   apply mor_subst.
 Qed.
 
-Fixpoint initial_morphism_unique {Sig : sig}(m : model Sig) (f : model_mor (ZModel Sig) m)
+Fixpoint initial_morphism_unique {S : signature}(m : model S) (f : model_mor (ZModel S) m)
      x : f x = initial_morphism m x. 
 Proof.
   destruct x.
